Update seq.dfy

seq.dfy
@@ -1,202 +1,294 @@
 predicate esteSolutie(solutie : seq<int>, nr:int)
-   requires |solutie| == 3
+   requires |solutie| == 4
    requires solutie[0]>=0
    requires solutie[1]>=0
    requires solutie[2]>=0
+   requires solutie[3]>=0
 {
-    solutie[0]*1+solutie[1]*5+solutie[2]*10 == nr
+    solutie[0]*1+solutie[1]*5+solutie[2]*10+solutie[3]*20 == nr
 
 }
 
 function cost(solutie : seq<int>):int 
-   requires |solutie| == 3
+   requires |solutie| == 4
    requires solutie[0]>=0
    requires solutie[1]>=0
    requires solutie[2]>=0
+   requires solutie[3]>=0
 {
-    solutie[0]+solutie[1]+solutie[2]
+    solutie[0]+solutie[1]+solutie[2]+solutie[3]
 }
 
 predicate esteSolutieOptima(solutie : seq<int>, nr:int)
-    requires |solutie| == 3
+    requires |solutie| == 4
     requires solutie[0]>=0
     requires solutie[1]>=0
     requires solutie[2]>=0
+    requires solutie[3]>=0
 {   
   esteSolutie(solutie,nr) &&
-  forall solutieOarecare :: |solutieOarecare| == 3 && solutieOarecare[0]>=0 && solutieOarecare[1]>=0 && solutieOarecare[2]>=0 && esteSolutie(solutieOarecare,nr) 
+  forall solutieOarecare :: |solutieOarecare| == 4 && solutieOarecare[0]>=0 && solutieOarecare[1]>=0 
+        && solutieOarecare[2]>=0 && solutieOarecare[3]>=0 && esteSolutie(solutieOarecare,nr) 
           ==> cost(solutieOarecare) >= cost(solutie)
 
 }
 
 predicate INV(copie: int, nr: int, solutieFinala : seq<int>)
-  requires |solutieFinala| == 3
+  requires |solutieFinala| == 4
   requires solutieFinala[0] >= 0
   requires solutieFinala[1] >= 0
   requires solutieFinala[2] >= 0
+  requires solutieFinala[3] >= 0
 {
-   forall solutieCurenta :: |solutieCurenta| == 3 && solutieCurenta[0] >= 0 && solutieCurenta[1] >=0 && solutieCurenta[2] >= 0 ==>
+   forall solutieCurenta :: |solutieCurenta| == 4 && solutieCurenta[0] >= 0 && solutieCurenta[1] >=0 && solutieCurenta[2]>=0 && solutieCurenta[3] >= 0 ==>
           (esteSolutie(solutieCurenta,copie) ==> 
-          esteSolutie([solutieFinala[0]+solutieCurenta[0],solutieFinala[1]+solutieCurenta[1],solutieFinala[2]+solutieCurenta[2]],nr)) &&
+          esteSolutie([solutieFinala[0]+solutieCurenta[0],solutieFinala[1]+solutieCurenta[1],solutieFinala[2]+solutieCurenta[2],solutieFinala[3]+solutieCurenta[3]],nr)) &&
           (esteSolutieOptima(solutieCurenta,copie) ==> 
-          esteSolutieOptima([solutieFinala[0]+solutieCurenta[0],solutieFinala[1]+solutieCurenta[1],solutieFinala[2]+solutieCurenta[2]],nr))
+          esteSolutieOptima([solutieFinala[0]+solutieCurenta[0],solutieFinala[1]+solutieCurenta[1],solutieFinala[2]+solutieCurenta[2],solutieFinala[3]+solutieCurenta[3]],nr))
 }
 
 
 method gasireMaxim(nr: int) returns(s:int)
   requires nr > 0
   ensures 0 < s <= nr
-  ensures s == 1 || s == 5 || s == 10
+  ensures s == 1 || s == 5 || s == 10 || s == 20
   ensures s == 1 ==> nr < 5
   ensures s == 5 ==> 5 <= nr < 10
-  ensures s == 10 ==> nr >= 10
-  
+  ensures s == 10 ==> 10 <= nr < 20
+  ensures s == 20 ==> nr >= 20
 {
-  if(nr >= 10){
-    s := 10;
-  }
-  else
-  {
-    if(nr >= 5){
-    s := 5;
-  }
-    else{
-       if(nr < 5){
-        s := 1; 
-        }
+    if(nr >= 20)
+    {
+        s := 20;
     }
-  }
-  
+    else if(nr >= 10){
+        s := 10;
+        }
+        else if(nr >= 5){
+        s := 5;
+            }
+            else if(nr < 5){
+                s := 1; 
+            }
+
 }
 
 
 lemma cazMaxim1(copie: int, nr: int, solutieFinala: seq<int>)
   requires copie < 5
-  requires |solutieFinala| == 3
+  requires |solutieFinala| == 4
   requires solutieFinala[0] >= 0
   requires solutieFinala[1] >= 0
   requires solutieFinala[2] >= 0
+  requires solutieFinala[3] >= 0
   requires INV(copie,nr,solutieFinala)
-  ensures INV(copie-1,nr,[(solutieFinala[0]+1),solutieFinala[1],solutieFinala[2]])
+  ensures INV(copie-1,nr,[(solutieFinala[0]+1),solutieFinala[1],solutieFinala[2],solutieFinala[3]])
 {
 
-  forall solutieCurenta | |solutieCurenta| == 3 && solutieCurenta[0] >= 0 && solutieCurenta[1] >=0 
-          && solutieCurenta[2] >= 0 && esteSolutieOptima(solutieCurenta,copie-1) 
+  forall solutieCurenta | |solutieCurenta| == 4 && solutieCurenta[0] >= 0 && solutieCurenta[1] >=0 
+          && solutieCurenta[2] >= 0  && solutieCurenta[3]>=0 && esteSolutieOptima(solutieCurenta,copie-1) 
           ensures esteSolutieOptima([solutieFinala[0]+solutieCurenta[0]+1,solutieFinala[1]+solutieCurenta[1],
-          solutieFinala[2]+solutieCurenta[2]],nr)
+          solutieFinala[2]+solutieCurenta[2],solutieFinala[3]+solutieCurenta[3]],nr)
   {
     assert esteSolutie(solutieCurenta,copie-1);
-    assert esteSolutie([solutieCurenta[0]+1,solutieCurenta[1],solutieCurenta[2]],copie);
+    assert esteSolutie([solutieCurenta[0]+1,solutieCurenta[1],solutieCurenta[2],solutieCurenta[3]],copie);
 
-    assert forall solutieOarecare :: |solutieOarecare| == 3 && solutieOarecare[0]>=0 && solutieOarecare[1]>=0 
-          && solutieOarecare[2]>=0 && esteSolutie(solutieOarecare,copie-1) 
+    assert forall solutieOarecare :: |solutieOarecare| == 4 && solutieOarecare[0]>=0 && solutieOarecare[1]>=0 
+          && solutieOarecare[2]>=0 && solutieOarecare[3]>=0 && esteSolutie(solutieOarecare,copie-1) 
           ==> cost(solutieOarecare) >= cost(solutieCurenta);
 
     assert esteSolutie([solutieFinala[0]+solutieCurenta[0]+1,solutieFinala[1]+solutieCurenta[1],
-          solutieFinala[2]+solutieCurenta[2]],nr);
+          solutieFinala[2]+solutieCurenta[2],solutieFinala[3]+solutieCurenta[3]],nr);
 
-    assert forall solutieOarecare :: |solutieOarecare| == 3 && solutieOarecare[0]>=0 && solutieOarecare[1]>=0 
-          && solutieOarecare[2]>=0 &&  esteSolutie(solutieOarecare,nr) 
+    assert forall solutieOarecare :: |solutieOarecare| == 4 && solutieOarecare[0]>=0 && solutieOarecare[1]>=0 
+          && solutieOarecare[2]>=0 && solutieOarecare[3]>=0 &&  esteSolutie(solutieOarecare,nr) 
           ==> cost(solutieOarecare) >= cost([solutieCurenta[0]+solutieFinala[0]+1,solutieCurenta[1]+solutieFinala[1],
-          solutieCurenta[2]+solutieFinala[2]]);
+          solutieCurenta[2]+solutieFinala[2],solutieCurenta[3]+solutieFinala[3]]);
   }
 
-  assert forall solutieCurenta :: |solutieCurenta|==3 && solutieCurenta[0]>=0 && solutieCurenta[1]>=0 && solutieCurenta[2]>=0 
+  assert forall solutieCurenta :: |solutieCurenta|==4 && solutieCurenta[0]>=0 && solutieCurenta[1]>=0 && solutieCurenta[2]>=0 && solutieCurenta[3]>=0 
           && esteSolutieOptima(solutieCurenta,copie-1) ==> 
           esteSolutieOptima([solutieFinala[0]+solutieCurenta[0]+1,solutieFinala[1]+solutieCurenta[1],
-          solutieFinala[2]+solutieCurenta[2]],nr);
+          solutieFinala[2]+solutieCurenta[2],solutieFinala[3]+solutieCurenta[3]],nr);
 
 }
 
 lemma cazMaxim5(copie: int, nr: int, solutieFinala: seq<int>)
   requires 5 <= copie < 10 
-  requires |solutieFinala| == 3
+  requires |solutieFinala| == 4
   requires solutieFinala[0] >= 0
   requires solutieFinala[1] >= 0
   requires solutieFinala[2] >= 0
+  requires solutieFinala[3] >= 0 
   requires INV(copie,nr,solutieFinala)
-  ensures INV(copie-5,nr,[solutieFinala[0],(solutieFinala[1]+1),solutieFinala[2]])
+  ensures INV(copie-5,nr,[solutieFinala[0],(solutieFinala[1]+1),solutieFinala[2],solutieFinala[3]])
 {
 
- forall solutieCurenta | |solutieCurenta| == 3 && solutieCurenta[0]>=0 && solutieCurenta[1]>=0 && 
-          solutieCurenta[2]>=0 && esteSolutieOptima(solutieCurenta,copie-5) 
+ forall solutieCurenta | |solutieCurenta| == 4 && solutieCurenta[0]>=0 && solutieCurenta[1]>=0 && 
+          solutieCurenta[2]>=0 && solutieCurenta[3]>=0 && esteSolutieOptima(solutieCurenta,copie-5) 
           ensures esteSolutieOptima([solutieFinala[0]+solutieCurenta[0],solutieFinala[1]+solutieCurenta[1]+1,
-          solutieCurenta[2]+solutieFinala[2]],nr)
+          solutieCurenta[2]+solutieFinala[2],solutieCurenta[3]+solutieFinala[3]],nr)
   {
     assert esteSolutie(solutieCurenta,copie-5);
-    assert esteSolutie([solutieCurenta[0], solutieCurenta[1]+1,solutieCurenta[2]],copie);
+    assert esteSolutie([solutieCurenta[0], solutieCurenta[1]+1,solutieCurenta[2],solutieCurenta[3]],copie);
 
-    assert forall solutieOarecare :: |solutieOarecare| == 3 && solutieOarecare[0]>=0 && solutieOarecare[1]>=0 && solutieOarecare[2]>=0 &&  esteSolutie(solutieOarecare,copie-5) 
+    assert forall solutieOarecare :: |solutieOarecare| == 4 && solutieOarecare[0]>=0 && solutieOarecare[1]>=0 &&
+          solutieOarecare[2]>=0 && solutieOarecare[3]>=0  && esteSolutie(solutieOarecare,copie-5) 
           ==> cost(solutieOarecare) >= cost(solutieCurenta);
-    assert esteSolutie([(solutieFinala[0]+solutieCurenta[0]),(solutieFinala[1]+solutieCurenta[1]+1),(solutieFinala[2]+solutieCurenta[2])],nr);
+    assert esteSolutie([solutieFinala[0]+solutieCurenta[0],solutieFinala[1]+solutieCurenta[1]+1,solutieFinala[2]+solutieCurenta[2],solutieFinala[3]+solutieCurenta[3]],nr);
     
-    assert forall solutieOarecare :: |solutieOarecare| == 3 && solutieOarecare[0]>=0 && solutieOarecare[1]>=0 && solutieOarecare[2]>=0 && esteSolutie(solutieOarecare,nr)
-          ==> cost(solutieOarecare) >= cost([solutieFinala[0]+solutieCurenta[0],solutieFinala[1]+solutieCurenta[1]+1,solutieFinala[2]+solutieCurenta[2]]);
+    assert forall solutieOarecare :: |solutieOarecare| == 4 && solutieOarecare[0]>=0 && solutieOarecare[1]>=0 && solutieOarecare[2]>=0 
+          && solutieOarecare[3]>=0 && esteSolutie(solutieOarecare,nr)
+          ==> cost(solutieOarecare) >= cost([solutieFinala[0]+solutieCurenta[0],solutieFinala[1]+solutieCurenta[1]+1,solutieFinala[2]+solutieCurenta[2],solutieFinala[3]+solutieCurenta[3]]);
   }
 
-  assert forall solutieCurenta :: |solutieCurenta| == 3 && solutieCurenta[0]>=0 && solutieCurenta[1]>=0 && solutieCurenta[2]>=0
-          && esteSolutie(solutieCurenta,copie-5) ==> 
-          esteSolutieOptima([solutieCurenta[0]+solutieFinala[0],solutieCurenta[1]+solutieFinala[1]+1,solutieCurenta[2]+solutieFinala[2]],nr);
+  assert forall solutieCurenta :: |solutieCurenta| == 4 && solutieCurenta[0]>=0 && solutieCurenta[1]>=0 && solutieCurenta[2]>=0
+          && solutieCurenta[3]>=0 && esteSolutie(solutieCurenta,copie-5) ==> 
+          esteSolutieOptima([solutieCurenta[0]+solutieFinala[0],solutieCurenta[1]+solutieFinala[1]+1,solutieCurenta[2]+solutieFinala[2],solutieCurenta[3]+solutieFinala[3]],nr);
+
+}
+
+lemma cazMaxim10(copie: int, nr: int, solutieFinala: seq<int>)
+  requires 10 <= copie < 20 
+  requires |solutieFinala| == 4
+  requires solutieFinala[0] >= 0
+  requires solutieFinala[1] >= 0
+  requires solutieFinala[2] >= 0
+  requires solutieFinala[3] >= 0 
+  requires INV(copie,nr,solutieFinala)
+  ensures INV(copie-10,nr,[solutieFinala[0],solutieFinala[1],solutieFinala[2]+1,solutieFinala[3]])
+{
+
+ forall solutieCurenta | |solutieCurenta| == 4 && solutieCurenta[0]>=0 && solutieCurenta[1]>=0 && 
+          solutieCurenta[2]>=0 && solutieCurenta[3]>=0 && esteSolutieOptima(solutieCurenta,copie-10) 
+          ensures esteSolutieOptima([solutieFinala[0]+solutieCurenta[0],solutieFinala[1]+solutieCurenta[1],
+          solutieCurenta[2]+solutieFinala[2]+1,solutieCurenta[3]+solutieFinala[3]],nr)
+  {
+    assert esteSolutie(solutieCurenta,copie-10);
+    assert esteSolutie([solutieCurenta[0], solutieCurenta[1],solutieCurenta[2]+1,solutieCurenta[3]],copie);
+
+    assert forall solutieOarecare :: |solutieOarecare| == 4 && solutieOarecare[0]>=0 && solutieOarecare[1]>=0 &&
+          solutieOarecare[2]>=0 && solutieOarecare[3]>=0  && esteSolutie(solutieOarecare,copie-10) 
+          ==> cost(solutieOarecare) >= cost(solutieCurenta);
+
+    assert esteSolutie([solutieFinala[0]+solutieCurenta[0],solutieFinala[1]+solutieCurenta[1],1+solutieFinala[2]+solutieCurenta[2],solutieFinala[3]+solutieCurenta[3]],nr);
+
+    assert forall solutieOarecare :: |solutieOarecare| == 4 && solutieOarecare[0]>=0 && solutieOarecare[1]>=0 
+            && solutieOarecare[2]>=0 && solutieOarecare[3]>=0 && esteSolutie(solutieOarecare,nr)
+          ==> cost(solutieOarecare) >= cost([solutieCurenta[0]+solutieFinala[0],solutieCurenta[1]+solutieFinala[1],
+                                        solutieCurenta[2]+solutieFinala[2]+1,solutieCurenta[3]+solutieFinala[3]]);
+  }
+
+  assert forall solutieCurenta :: |solutieCurenta| == 4 && solutieCurenta[0]>=0 && solutieCurenta[1]>=0 && solutieCurenta[2]>=0
+          && solutieCurenta[3]>=0 && esteSolutie(solutieCurenta,copie-10) ==> 
+          esteSolutieOptima([solutieCurenta[0]+solutieFinala[0],solutieCurenta[1]+solutieFinala[1],
+                            solutieCurenta[2]+solutieFinala[2]+1,solutieCurenta[3]+solutieFinala[3]],nr);
 
 }
 
 
+
 lemma B(copie:int,nr: int,solutieOarecare : seq<int>, solutieCurenta: seq<int>)
-  requires |solutieOarecare| == 3
+  requires |solutieOarecare| == 4
   requires solutieOarecare[0]>=0
   requires solutieOarecare[1]>=0
   requires solutieOarecare[2]>=0
-  requires |solutieCurenta| == 3
+  requires solutieOarecare[3]>=0
+  requires |solutieCurenta| == 4
   requires solutieCurenta[0] >= 0
   requires solutieCurenta[1] >= 0
-  requires solutieCurenta[2] >=0
-  requires copie >=10
+  requires solutieCurenta[2] >= 0
+  requires solutieCurenta[3] >= 0
+  requires copie >= 20
   requires esteSolutie(solutieOarecare,copie)
-  requires esteSolutie(solutieCurenta,copie-10)
-  requires esteSolutieOptima(solutieCurenta,copie-10)
-  ensures cost(solutieOarecare) >= cost([solutieCurenta[0],solutieCurenta[1],(solutieCurenta[2]+1)])
-  decreases solutieOarecare[0],solutieOarecare[1]
+  requires esteSolutie(solutieCurenta,copie-20)
+  requires esteSolutieOptima(solutieCurenta,copie-20)
+  ensures cost(solutieOarecare) >= cost([solutieCurenta[0],solutieCurenta[1],solutieCurenta[2],1+solutieCurenta[3]])
+  decreases solutieOarecare[0],solutieOarecare[1],solutieOarecare[2]
 {
   assert esteSolutie(solutieOarecare,copie);
-  assert esteSolutie([solutieCurenta[0],solutieCurenta[1],(solutieCurenta[2]+1)],copie);
+  assert esteSolutie([solutieCurenta[0],solutieCurenta[1],solutieCurenta[2],solutieCurenta[3]+1],copie);
 
-  if(cost(solutieOarecare) < cost([solutieCurenta[0],solutieCurenta[1],(solutieCurenta[2]+1)]))
+  if(cost(solutieOarecare) < cost([solutieCurenta[0],solutieCurenta[1],solutieCurenta[2],1+solutieCurenta[3]]))
   {
-    if(solutieOarecare[2] > (solutieCurenta[2]+1))
+    if(solutieOarecare[3] > (solutieCurenta[3]+1))
     {
-      assert cost([solutieOarecare[0],solutieOarecare[1],(solutieOarecare[2]-1)]) < cost(solutieCurenta);
-      assert esteSolutieOptima([solutieOarecare[0],solutieOarecare[1],(solutieOarecare[2]-1)],(copie-10));
+      assert cost([solutieOarecare[0],solutieOarecare[1],solutieOarecare[2],solutieOarecare[3]-1]) < cost(solutieCurenta);
+      assert esteSolutieOptima([solutieOarecare[0],solutieOarecare[1],solutieOarecare[2],solutieOarecare[3]-1],(copie-20));
+      assert false;
+      
+    }
+    else if(solutieOarecare[3] < solutieCurenta[3]+1)
+      {
+        assert (solutieOarecare[0]+(5*solutieOarecare[1])+(10*solutieOarecare[2]))>20;
+        
+        if(solutieOarecare[0]>=20)
+        {
+          var nouaSolutieOarecare := [solutieOarecare[0]-20,solutieOarecare[1],solutieOarecare[2],solutieOarecare[3]+1];
+          B(copie,nr,nouaSolutieOarecare, solutieCurenta);
+        }
+        else if(solutieOarecare[0]>=15 && solutieOarecare[1]>=1){
+               var nouaSolutieOarecare := [solutieOarecare[0]-15,solutieOarecare[1]-1,solutieOarecare[2],solutieOarecare[3]+1];
+                B(copie,nr,nouaSolutieOarecare, solutieCurenta);
+        }
+        else if(solutieOarecare[0]>=10 && solutieOarecare[1]>=2){
+               var nouaSolutieOarecare := [solutieOarecare[0]-10,solutieOarecare[1]-2,solutieOarecare[2],solutieOarecare[3]+1];
+                B(copie,nr,nouaSolutieOarecare, solutieCurenta);
+        }
+        else if(solutieOarecare[0]>=10 && solutieOarecare[2]>=1){
+               var nouaSolutieOarecare := [solutieOarecare[0]-10,solutieOarecare[1],solutieOarecare[2]-1,solutieOarecare[3]+1];
+                B(copie,nr,nouaSolutieOarecare, solutieCurenta);
+        }
+        else if(solutieOarecare[0]>=5 && solutieOarecare[1]>=3){
+               var nouaSolutieOarecare := [solutieOarecare[0]-5,solutieOarecare[1]-3,solutieOarecare[2],solutieOarecare[3]+1];
+                B(copie,nr,nouaSolutieOarecare, solutieCurenta);
+        }
+        else if(solutieOarecare[0]>=5 && solutieOarecare[1]>=1 && solutieOarecare[2]>=1){
+               var nouaSolutieOarecare := [solutieOarecare[0]-5,solutieOarecare[1]-1,solutieOarecare[2]-1,solutieOarecare[3]+1];
+                B(copie,nr,nouaSolutieOarecare, solutieCurenta);
+        }
+        else if(solutieOarecare[1]>=2 && solutieOarecare[2]>=1){
+               var nouaSolutieOarecare := [solutieOarecare[0],solutieOarecare[1]-2,solutieOarecare[2]-1,solutieOarecare[3]+1];
+                B(copie,nr,nouaSolutieOarecare, solutieCurenta);
+        }
+        else{
+               var nouaSolutieOarecare := [solutieOarecare[0],solutieOarecare[1],solutieOarecare[2]-2,solutieOarecare[3]+1];
+                B(copie,nr,nouaSolutieOarecare, solutieCurenta);
+        }
+        
+      }
+
+    assert solutieOarecare[3] == (solutieCurenta[3]+1);
+
+    if(solutieOarecare[2]>solutieCurenta[2])
+    {
+      assert cost([solutieOarecare[0],solutieOarecare[1],solutieOarecare[2],solutieOarecare[3]-1]) < cost(solutieCurenta);
       assert false;
     }
-    else
-    {
-      if(solutieOarecare[2] < solutieCurenta[2]+1)
+    else if(solutieOarecare[2] < solutieCurenta[2])
       {
         assert (solutieOarecare[0]+(5*solutieOarecare[1]))>10;
 
         if(solutieOarecare[0]>=10)
         {
-          var sol'' := [solutieOarecare[0]-10,solutieOarecare[1],solutieOarecare[2]+1];
-          B(copie,nr,sol'', solutieCurenta);
+          var nouaSolutieOarecare := [solutieOarecare[0]-10,solutieOarecare[1],solutieOarecare[2]+1,solutieOarecare[3]];
+          B(copie,nr,nouaSolutieOarecare, solutieCurenta);
         }
-        else{
-          if(solutieOarecare[1]>=2){
-            var sol'' := [solutieOarecare[0],solutieOarecare[1]-2,solutieOarecare[2]+1];
-             B(copie,nr,sol'', solutieCurenta);
-          }
+        else if(solutieOarecare[1]>=2){
+            var nouaSolutieOarecare := [solutieOarecare[0],solutieOarecare[1]-2,solutieOarecare[2]+1,solutieOarecare[3]];
+             B(copie,nr,nouaSolutieOarecare, solutieCurenta);
+        }
           else
           {
-            var sol'' := [solutieOarecare[0]-5,solutieOarecare[1]-1,solutieOarecare[2]+1];
-             B(copie,nr,sol'', solutieCurenta);
+            var nouaSolutieOarecare := [solutieOarecare[0]-5,solutieOarecare[1]-1,solutieOarecare[2]+1,solutieOarecare[3]];
+             B(copie,nr,nouaSolutieOarecare, solutieCurenta);
           }
         }
-      }
-    }
-    assert solutieOarecare[2] == (solutieCurenta[2]+1);
+        assert solutieOarecare[2] == solutieCurenta[2];
 
-    if(solutieOarecare[1]>solutieCurenta[1])
+      if(solutieOarecare[1]>solutieCurenta[1])
     {
-      assert cost([solutieOarecare[0],solutieOarecare[1],(solutieOarecare[2]-1)]) < cost(solutieCurenta);
+      assert cost([solutieOarecare[0],solutieOarecare[1],solutieOarecare[2],solutieOarecare[3]-1]) < cost(solutieCurenta);
       assert false;
     }
     else
@@ -205,33 +297,31 @@ lemma B(copie:int,nr: int,solutieOarecare : seq<int>, solutieCurenta: seq<int>)
       {
         assert solutieOarecare[0]>=5;
       
-          var sol'' := [solutieOarecare[0]-5,solutieOarecare[1]+1,solutieOarecare[2]];
-          B(copie, nr, sol'', solutieCurenta);
+          var nouaSolutieOarecare := [solutieOarecare[0]-5,solutieOarecare[1]+1,solutieOarecare[2],solutieOarecare[3]];
+          B(copie, nr, nouaSolutieOarecare, solutieCurenta);
         
       }
     }
-
-    assert solutieOarecare[1] == solutieCurenta[1];
-
     assert solutieOarecare[0]==solutieCurenta[0];
-    
     assert false;
+
   }
 }
 
 lemma esteSolutiePentruCopie(copie:int,nr: int, solutieCurenta:seq<int>)
-  requires |solutieCurenta| == 3
+  requires |solutieCurenta| == 4
   requires solutieCurenta[0] >= 0
   requires solutieCurenta[1] >= 0
   requires solutieCurenta[2] >= 0
-  requires copie >= 10
-  requires esteSolutie(solutieCurenta,copie-10)
-  requires esteSolutieOptima(solutieCurenta,copie-10)
-  ensures esteSolutieOptima([solutieCurenta[0],solutieCurenta[1],solutieCurenta[2]+1],copie)
+  requires solutieCurenta[3] >= 0
+  requires copie >= 20
+  requires esteSolutie(solutieCurenta,copie-20)
+  requires esteSolutieOptima(solutieCurenta,copie-20)
+  ensures esteSolutieOptima([solutieCurenta[0],solutieCurenta[1],solutieCurenta[2],1+solutieCurenta[3]],copie)
 {
-  forall solutieOarecare | |solutieOarecare| == 3 && solutieOarecare[0]>=0 && solutieOarecare[1]>=0 && 
-        solutieOarecare[2]>=0 && esteSolutie(solutieOarecare,copie)
-    ensures cost(solutieOarecare)>=cost([solutieCurenta[0],solutieCurenta[1],(solutieCurenta[2]+1)])
+  forall solutieOarecare | |solutieOarecare| == 4 && solutieOarecare[0]>=0 && solutieOarecare[1]>=0 && 
+        solutieOarecare[2]>=0 && solutieOarecare[3]>=0 && esteSolutie(solutieOarecare,copie)
+    ensures cost(solutieOarecare)>=cost([solutieCurenta[0],solutieCurenta[1],solutieCurenta[2],1+solutieCurenta[3]])
   {
     B(copie,nr, solutieOarecare, solutieCurenta);
   }
@@ -239,24 +329,27 @@ lemma esteSolutiePentruCopie(copie:int,nr: int, solutieCurenta:seq<int>)
 }
 
 lemma aux(copie: int ,nr: int, solutieOarecare : seq<int>, solutieFinala : seq<int>, solutieCurenta:seq<int>)
-  requires |solutieOarecare| == 3
+  requires |solutieOarecare| == 4
   requires solutieOarecare[0]>=0
   requires solutieOarecare[1]>=0
   requires solutieOarecare[2]>=0
-  requires |solutieFinala| == 3
+  requires solutieOarecare[3]>=0
+  requires |solutieFinala| == 4
   requires solutieFinala[0] >= 0
   requires solutieFinala[1] >= 0
   requires solutieFinala[2] >= 0
-  requires |solutieCurenta| == 3
+  requires solutieFinala[3] >= 0
+  requires |solutieCurenta| == 4
   requires solutieCurenta[0] >= 0 
   requires solutieCurenta[1] >= 0
   requires solutieCurenta[2] >= 0
-  requires copie >= 10 
-  requires esteSolutieOptima(solutieCurenta,copie-10)
-  requires esteSolutie([solutieFinala[0]+solutieCurenta[0],solutieFinala[1]+solutieCurenta[1],solutieFinala[2]+solutieCurenta[2]+1],nr)
+  requires solutieCurenta[3] >= 0
+  requires copie >= 20
+  requires esteSolutieOptima(solutieCurenta,copie-20)
+  requires esteSolutie([solutieFinala[0]+solutieCurenta[0],solutieFinala[1]+solutieCurenta[1],solutieFinala[2]+solutieCurenta[2],1+solutieFinala[3]+solutieCurenta[3]],nr)
   requires esteSolutie(solutieOarecare,nr)
   requires INV(copie,nr,solutieFinala)
-  ensures cost(solutieOarecare) >= cost([solutieFinala[0]+solutieCurenta[0],solutieFinala[1]+solutieCurenta[1],solutieFinala[2]+solutieCurenta[2]+1])
+  ensures cost(solutieOarecare) >= cost([solutieFinala[0]+solutieCurenta[0],solutieFinala[1]+solutieCurenta[1],solutieFinala[2]+solutieCurenta[2],1+solutieFinala[3]+solutieCurenta[3]])
 {
   esteSolutiePentruCopie(copie,nr,solutieCurenta);
 }
@@ -264,126 +357,134 @@ lemma aux(copie: int ,nr: int, solutieOarecare : seq<int>, solutieFinala : seq<i
 
 
 
-lemma cazMaxim10(copie: int,nr: int, solutieFinala : seq<int>)
-  requires copie >= 10
-  requires |solutieFinala| == 3
+lemma cazMaxim20(copie: int,nr: int, solutieFinala : seq<int>)
+  requires copie >= 20
+  requires |solutieFinala| == 4
   requires solutieFinala[0] >= 0
   requires solutieFinala[1] >= 0
   requires solutieFinala[2] >= 0
+  requires solutieFinala[3] >= 0
   requires INV(copie,nr,solutieFinala)
-  ensures INV(copie-10,nr,[solutieFinala[0],solutieFinala[1],(solutieFinala[2]+1)])
+  ensures INV(copie-20,nr,[solutieFinala[0],solutieFinala[1],solutieFinala[2],solutieFinala[3]+1])
 {
-  assert forall solutieCurenta :: |solutieCurenta|==3 && solutieCurenta[0]>=0 && solutieCurenta[1]>=0 && solutieCurenta[2]>=0 ==>
+  assert forall solutieCurenta :: |solutieCurenta|==4  && solutieCurenta[0]>=0 && solutieCurenta[1]>=0 && solutieCurenta[2]>=0 && solutieCurenta[3]>=0 ==>
           (esteSolutie(solutieCurenta,copie) ==> 
-          esteSolutie([solutieFinala[0]+solutieCurenta[0],solutieFinala[1]+solutieCurenta[1],solutieFinala[2]+solutieCurenta[2]],nr));
+          esteSolutie([solutieFinala[0]+solutieCurenta[0],solutieFinala[1]+solutieCurenta[1],solutieFinala[2]+solutieCurenta[2],solutieFinala[3]+solutieCurenta[3]],nr));
 
-   forall solutieCurenta | |solutieCurenta| == 3  && solutieCurenta[0]>=0 && solutieCurenta[1]>=0 && solutieCurenta[2]>=0 
-          && esteSolutie(solutieCurenta,copie-10) 
-          ensures esteSolutie([solutieFinala[0]+solutieCurenta[0],solutieFinala[1]+solutieCurenta[1],solutieFinala[2]+solutieCurenta[2]+1],nr)
+   forall solutieCurenta | |solutieCurenta| == 4  && solutieCurenta[0]>=0 && solutieCurenta[1]>=0 && solutieCurenta[2]>=0 && solutieCurenta[3]>=0 
+          && esteSolutie(solutieCurenta,copie-20) 
+          ensures esteSolutie([solutieFinala[0]+solutieCurenta[0],solutieFinala[1]+solutieCurenta[1],solutieFinala[2]+solutieCurenta[2],solutieFinala[3]+solutieCurenta[3]+1],nr)
    {
-     assert esteSolutie([solutieCurenta[0],solutieCurenta[1],solutieCurenta[2]+1],copie);
+     assert esteSolutie([solutieCurenta[0],solutieCurenta[1],solutieCurenta[2],solutieCurenta[3]+1],copie);
    }
   
 
-  forall solutieCurenta | |solutieCurenta|==3 && solutieCurenta[0]>=0 && solutieCurenta[1]>=0 && solutieCurenta[2]>=0 >= 0 
-          && esteSolutieOptima(solutieCurenta,copie-10) 
-          ensures esteSolutieOptima([solutieFinala[0]+solutieCurenta[0],solutieFinala[1]+solutieCurenta[1],solutieFinala[2]+solutieCurenta[2]+1],nr)
+  forall solutieCurenta | |solutieCurenta|==4 && solutieCurenta[0]>=0 && solutieCurenta[1]>=0 && solutieCurenta[2]>=0 && solutieCurenta[3]>=0 
+          && esteSolutieOptima(solutieCurenta,copie-20) 
+          ensures esteSolutieOptima([solutieFinala[0]+solutieCurenta[0],solutieFinala[1]+solutieCurenta[1],solutieFinala[2]+solutieCurenta[2],solutieFinala[3]+solutieCurenta[3]+1],nr)
   {
 
-    assert esteSolutie(solutieCurenta,copie-10);
-    assert esteSolutie([solutieCurenta[0],solutieCurenta[1],solutieCurenta[2]+1],copie);
+    assert esteSolutie(solutieCurenta,copie-20);
+    assert esteSolutie([solutieCurenta[0],solutieCurenta[1],solutieCurenta[2],solutieCurenta[3]+1],copie);
 
-    assert forall solutieOarecare :: |solutieOarecare| == 3 && solutieOarecare[0]>=0 && solutieOarecare[1]>=0 && solutieOarecare[2]>=0
-          && esteSolutie(solutieOarecare,copie-10) 
+    assert forall solutieOarecare :: |solutieOarecare| == 4 && solutieOarecare[0]>=0 && solutieOarecare[1]>=0 && solutieOarecare[2]>=0 && solutieOarecare[3]>=0
+          && esteSolutie(solutieOarecare,copie-20) 
           ==> cost(solutieOarecare) >= cost(solutieCurenta);
 
 
-    assert esteSolutie([solutieFinala[0]+solutieCurenta[0],solutieFinala[1]+solutieCurenta[1],solutieFinala[2]+solutieCurenta[2]+1],nr);
+    assert esteSolutie([solutieFinala[0]+solutieCurenta[0],solutieFinala[1]+solutieCurenta[1],solutieFinala[2]+solutieCurenta[2],solutieFinala[3]+solutieCurenta[3]+1],nr);
 
-    forall solutieOarecare | |solutieOarecare| == 3 && solutieOarecare[0]>=0 && solutieOarecare[1]>=0 && solutieOarecare[2]>=0 
+    forall solutieOarecare | |solutieOarecare| == 4 && solutieOarecare[0]>=0 && solutieOarecare[1]>=0 && solutieOarecare[2]>=0 && solutieOarecare[3]>=0
                  && esteSolutie(solutieOarecare,nr)
-      ensures cost(solutieOarecare) >= cost([solutieFinala[0]+solutieCurenta[0],solutieFinala[1]+solutieCurenta[1],solutieFinala[2]+solutieCurenta[2]+1])
+      ensures cost(solutieOarecare) >= cost([solutieFinala[0]+solutieCurenta[0],solutieFinala[1]+solutieCurenta[1],solutieFinala[2]+solutieCurenta[2],1+solutieFinala[3]+solutieCurenta[3]])
       {
           aux(copie, nr, solutieOarecare, solutieFinala, solutieCurenta);
       }
 
-    assert forall solutieOarecare :: |solutieOarecare| == 3 && solutieOarecare[0]>=0 && solutieOarecare[1]>=0 && solutieOarecare[2]>=0
+    assert forall solutieOarecare :: |solutieOarecare| == 4 && solutieOarecare[0]>=0 && solutieOarecare[1]>=0 && solutieOarecare[2]>=0 && solutieOarecare[3]>=0
              && esteSolutie(solutieOarecare,nr) 
-          ==> cost(solutieOarecare) >= cost([solutieFinala[0]+solutieCurenta[0],solutieFinala[1]+solutieCurenta[1],(solutieFinala[2]+solutieCurenta[2]+1)]);
+          ==> cost(solutieOarecare) >= cost([solutieFinala[0]+solutieCurenta[0],solutieFinala[1]+solutieCurenta[1],solutieFinala[2]+solutieCurenta[2],1+solutieFinala[3]+solutieCurenta[3]]);
   }
 
 
-  assert forall solutieCurenta :: |solutieCurenta|==3 && solutieCurenta[0]>=0 && solutieCurenta[1]>=0 && solutieCurenta[2]>=0
-          && esteSolutieOptima(solutieCurenta,copie-10) ==> 
-          esteSolutieOptima([solutieFinala[0]+solutieCurenta[0],solutieFinala[1]+solutieCurenta[1],solutieFinala[2]+solutieCurenta[2]+1],nr);
+  assert forall solutieCurenta :: |solutieCurenta| == 4 && solutieCurenta[0]>=0 && solutieCurenta[1]>=0 && solutieCurenta[2]>=0 && solutieCurenta[3]>=0
+          && esteSolutieOptima(solutieCurenta,copie-20) ==> 
+          esteSolutieOptima([solutieFinala[0]+solutieCurenta[0],solutieFinala[1]+solutieCurenta[1],solutieFinala[2]+solutieCurenta[2],1+solutieFinala[3]+solutieCurenta[3]],nr);
 
 
-  assert forall solutieCurenta :: |solutieCurenta| == 3 && solutieCurenta[0]>=0 && solutieCurenta[1]>=0 && solutieCurenta[2]>=0 ==>
-          (esteSolutie(solutieCurenta,copie-10) ==> 
-          esteSolutie([solutieFinala[0]+solutieCurenta[0],solutieFinala[1]+solutieCurenta[1],solutieFinala[2]+solutieCurenta[2]+1],nr));
+  assert forall solutieCurenta :: |solutieCurenta| == 4 && solutieCurenta[0]>=0 && solutieCurenta[1]>=0 && solutieCurenta[2]>=0 && solutieCurenta[3]>=0 ==>
+          (esteSolutie(solutieCurenta,copie-20) ==> 
+          esteSolutie([solutieFinala[0]+solutieCurenta[0],solutieFinala[1]+solutieCurenta[1],solutieFinala[2]+solutieCurenta[2],1+solutieFinala[3]+solutieCurenta[3]],nr));
   
-  assert forall solutieCurenta :: |solutieCurenta| == 3 && solutieCurenta[0]>=0 && solutieCurenta[1]>=0 && solutieCurenta[2]>=0 ==>        
-          (esteSolutieOptima(solutieCurenta,copie-10) ==> 
-          esteSolutieOptima([solutieFinala[0]+solutieCurenta[0],solutieFinala[1]+solutieCurenta[1],solutieFinala[2]+solutieCurenta[2]+1],nr));
+  assert forall solutieCurenta :: |solutieCurenta| == 4 && solutieCurenta[0]>=0 && solutieCurenta[1]>=0 && solutieCurenta[2]>=0 && solutieCurenta[3] >= 0 ==>        
+          (esteSolutieOptima(solutieCurenta,copie-20) ==> 
+          esteSolutieOptima([solutieFinala[0]+solutieCurenta[0],solutieFinala[1]+solutieCurenta[1],solutieFinala[2]+solutieCurenta[2],solutieFinala[3]+solutieCurenta[3]+1],nr));
 
-  assert  INV(copie-10,nr,[solutieFinala[0],solutieFinala[1],(solutieFinala[2]+1)]);
+  assert  INV(copie-20,nr,[solutieFinala[0],solutieFinala[1],solutieFinala[2],1+solutieFinala[3]]);
 }
 
 
 
   method nrMinimBancnote(nr: int) returns (solutie: seq<int>)
     requires nr>=0
-    ensures |solutie| == 3
+    ensures |solutie| == 4
     ensures solutie[0]>=0
     ensures solutie[1]>=0
     ensures solutie[2]>=0
+    ensures solutie[3]>=0
     ensures esteSolutie(solutie,nr)
-    ensures esteSolutie(solutie,nr)
+    ensures esteSolutieOptima(solutie,nr)
 {
 
     var copie:=  nr;
     var s1 := 0;
     var s5 := 0;
     var s10 := 0;
+    var s20 := 0;
     while(copie > 0)
       decreases copie
       invariant 0<=copie<=nr
-      invariant esteSolutie([s1,s5,s10],nr-copie)
-      invariant INV(copie,nr,[s1,s5,s10])
+      invariant esteSolutie([s1,s5,s10,s20],nr-copie)
+      invariant INV(copie,nr,[s1,s5,s10,s20])
     {
         var i := 0;
         var s := gasireMaxim(copie);
         if( s == 1){
-            cazMaxim1(copie,nr,[s1,s5,s10]);
+            cazMaxim1(copie,nr,[s1,s5,s10,s20]);
             s1:=s1+1;
-            assert esteSolutie([s1,s5,s10],nr-(copie-1));
-            assert INV(copie-1,nr,[s1,s5,s10]);
+            assert esteSolutie([s1,s5,s10,s20],nr-(copie-1));
+            assert INV(copie-1,nr,[s1,s5,s10,s20]);
         }
-        else{
-            if(s == 5)
+        else if(s == 5)
             {
-                cazMaxim5(copie,nr,[s1,s5,s10]);
+                cazMaxim5(copie,nr,[s1,s5,s10,s20]);
                 s5:=s5+1;
-                assert esteSolutie([s1,s5,s10],nr-(copie-5));
-                assert INV(copie-5,nr,[s1,s5,s10]);
+                assert esteSolutie([s1,s5,s10,s20],nr-(copie-5));
+                assert INV(copie-5,nr,[s1,s5,s10,s20]);
+
+            }
+            else if (s == 10){
+                cazMaxim10(copie,nr,[s1,s5,s10,s20]);
+                s10:=s10+1;
+                assert esteSolutie([s1,s5,s10,s20],nr-(copie-10));
+                assert INV(copie-10,nr,[s1,s5,s10,s20]);
 
             }
             else{
-                cazMaxim10(copie,nr,[s1,s5,s10]);
-                s10:=s10+1;
-                assert esteSolutie([s1,s5,s10],nr-(copie-10));
-                assert INV(copie-10,nr,[s1,s5,s10]);
-
+                cazMaxim20(copie,nr,[s1,s5,s10,s20]);
+                s20:=s20+1;
+                assert esteSolutie([s1,s5,s10,s20],nr-(copie-20));
+                assert INV(copie-20,nr,[s1,s5,s10,s20]);
             }
-        }
+
         copie := copie-s;
     }
-    solutie := [s1,s5,s10];
+    solutie := [s1,s5,s10,s20];
 }
 
 
 method Main() {
-  var nr:= 58;
+  var nr:= 18;
   var sol:=nrMinimBancnote(nr);
   print sol;
 }
